Test/dafny0/Computations.dfy
@@ -150,3 +150,20 @@ ghost method copt_test()
   ensures copt(Plus(Plus(Plus(Num(0), Num(0)), Num(0)), Num(1)))==Num(1);
 {
 }
+
+// The following is a test that well-typedness antecednets are included in the literal axioms
+static function StaticFact(n: nat): nat
+  ensures 0 < StaticFact(n);
+{
+  if n == 0 then 1 else n * StaticFact(n - 1)
+}
+static method test_StaticFact()
+{
+  assert StaticFact(0) == 1;
+  assert 42 != 42;  // error:  this should fail
+} 
+method test_fact()
+{
+  assert fact(0) == 1;
+  assert 42 != 42;  // error:  this should fail
+} 
